\section{Αποδειξεις}
%\begin{multicols}{2}[\section{Αποδειξεις}]

\subsection{Jackson recursion}
\begin{equation}
\begin{split}
    G_{4:0} &= g_4 + p_4    g_3 + p_4p_3g_2 + p_4p_3p_2g_1 + p_4p_3p_2p_1g_0 \\\
            &= p_4\bigg[g_4 + g_3 + p_3g_2 + p_3p_2g_1 + p_3p_2p_1g_0\bigg] \\
            &= p_4\bigg[g_4 + p_3\Big[ g_3 + g_2 + p_2g_1 + p_2p_1g_0\Big]\bigg] \\
            &= p_4g_4 + p_4p_3\bigg[ g_3 + g_2 + p_2g_1 + p_2p_1g_0\bigg] \\
            &= g_4 + p_4p_3\bigg[ g_3 + g_2 + p_2g_1 + p_2p_1g_0\bigg] \\
            \text{\textcolor{red}{Note}}&: \textcolor{red}{x+y*z=(x+y)*(x+z)}   \\
            &=\bigg[g_4 + p_4p_3\bigg]\bigg[g_4 + g_3 + g_2 + p_2g_1 + p_2p_1g_0\bigg] \\
            &= p_4\bigg[g_4 + p_3\Big[ g_3 + g_2 + p_2g_1 + p_2p_1g_0 \Big]\bigg] \\
            &= p_4\bigg[g_4 + p_3\Big[ g_3 + p_2( g_2 + g_1 + p_1g_0 )\Big]\bigg] \\
            &= p_4\bigg[g_4 + p_3g_3 + p_3p_2\Big[ g_2 + g_1 + p_1g_0 \Big]\bigg] \\  
            &= p_4\bigg[g_4 + \Big[ p_3g_3 + p_3p_2 \Big]\Big[ p_3g_3 + g_2 + g_1 + p_1g_0 \Big]    \bigg] \\
            &= p_4g_4 + p_4\Big[ g_3 + p_3p_2 \Big]\Big[ g_3 + g_2 + g_1 + p_1g_0 \Big]  \\
            &= g_4 + \Big[ p_4g_3 + p_4p_3p_2 \Big]\Big[ g_3 + g_2 + g_1 + p_1g_0 \Big]  \\ 
            &= \Big[g_4 +  p_4g_3 + p_4p_3p_2 \Big]\Big[ g_4 + g_3 + g_2 + g_1 + p_1g_0 \Big]
\end{split}
\end{equation}

\subsection{Jackson D}
\begin{equation}
\begin{split}
    D_{i:k} &= G_{j:k} + P_{j:k}\\
            &= G_{j:k+1} + P_{j:k-1}g_k  + P_{j:k}\\
            &= G_{j:k+1} + P_{j:k-1}g_k  + P_{j:k-1}p_k\\
            &= G_{j:k+1} + P_{j:k-1}(g_k + p_k)\\
            &= G_{j:k+1} + P_{j:k-1}( a_kb_k + a_k + b_k )\\
            &= G_{j:k+1} + P_{j:k-1}( a_k(b_k + 1) + b_k )\\
            &= G_{j:k+1} + P_{j:k-1}( a_k + b_k )\\
            &= G_{j:k+1} + P_{j:k-1}p_k \\
            &= G_{j:k+1} + P_{j:k}
\end{split}
\end{equation}

%\end{multicols}